Clean/Circuit/LookupCircuit.lean
@@ -23,9 +23,8 @@ def proverEnvironment (circuit : LookupCircuit F α β) (input : α F) : Environ
 theorem proverEnvironment_uses_local_witnesses (circuit : LookupCircuit F α β) (input : α F) :
     (circuit.proverEnvironment input).uses_local_witnesses 0 ((circuit.main (const input)).operations 0) := by
   apply Circuit.proverEnvironment_uses_local_witnesses
-  intro env env'
-  apply circuit.computableWitnesses 0 (const input)
-  simp only [Environment.agreesBelow, ProvableType.eval_const, implies_true]
+  apply circuit.compose_computableWitnesses
+  simp [Environment.onlyAccessedBelow, ProvableType.eval_const, circuit.computableWitnesses]
 
 def constantOutput (circuit : LookupCircuit F α β) (input : α F) : β F :=
   circuit.output (const input) 0 |> eval (circuit.proverEnvironment input)
