Clean/Gadgets/Addition8/Addition8FullCarry.lean
@@ -135,16 +135,9 @@ def lookupCircuit : LookupCircuit (F p) Inputs Outputs := {
   circuit with
   name := "Addition8FullCarry"
 
-  -- TODO this is not very hard, but it could be made even easier with a tactic script,
-  -- or even just restructuring the statement to include the inputs hypothesis in _every_ subgoal
   computableWitnesses n input := by
     simp_all only [circuit_norm, subcircuit_norm, circuit, add8_full_carry, Boolean.circuit,
-      Operations.forAllFlat, FlatOperation.forAll, Operations.toFlat,
-      Operations.computableWitnesses, Environment.agreesBelow,
-      Inputs.mk.injEq, Array.mk.injEq, List.cons.injEq]
-    intro env env' h_input env_agrees_below
-    specialize h_input (Environment.agreesBelow_of_le env_agrees_below (by linarith))
-    simp_all
+      Operations.forAllFlat, Operations.toFlat, FlatOperation.forAll, Inputs.mk.injEq]
 }
 
 end Gadgets.Addition8FullCarry
